updated lifted predicates

deps/poulet4/lib/P4cub/Transformations/Lifting/Lifted.v
@@ -4,6 +4,12 @@ Require Export Poulet4.P4cub.Syntax.Syntax
         Coq.Strings.Ascii Coq.Strings.String.
 Import AllCubNotations StringSyntax Field.FieldTactics.
 
+Ltac pair_destr :=
+  match goal with
+  | h: (_,_) = (_,_) |- _ => inv h
+  end.
+
+(*
 Ltac translateParserExpr_destr :=
   match goal with 
   | |- context [TranslateParserExpr ?e ?env]
@@ -15,13 +21,15 @@ Ltac translateCases'_destr :=
   | |- context [TranslateCases' ?c ?env ?i]
     => destruct (TranslateCases' c env i) as [[? ?] ?] eqn:?; simpl in *
   end.
-
+ *)
+(*
 Ltac translateStmt_destr :=
   match goal with
   | |- context [TranslateStatement ?s ?env]
     => destruct (TranslateStatement s env) as [? ?] eqn:?; simpl in *
   end.
-
+ *)
+(*
 Ltac translateArrowE_destr :=
   match goal with
   | |- context [TranslateArrowE ?args ?env ?i]
@@ -33,17 +41,15 @@ Ltac translateArgs_destr :=
   | |- context [TranslateArgs ?args ?env ?i]
     => destruct (TranslateArgs args env i) as [[? ?] ?] eqn:?; simpl in *
   end.
+*)
 
-Ltac transformExpr_destr :=
+Ltac lift_e_destr :=
   match goal with
-  | |- context [TransformExpr ?e ?env]
-    => destruct (TransformExpr e env) as [[? ?] ?] eqn:?; simpl in *
-  | |- context [TransformExprList' ?f ?e ?env ?i]
-    => destruct (TransformExprList' f e env i) as [[? ?] ?] eqn:?; simpl in *
-  | |- context [TransformFields' ?f ?e ?env ?i]
-    => destruct (TransformFields' f e env i) as [[? ?] ?] eqn:?; simpl in *
+  | |- context [lift_e ?up ?e]
+    => destruct (lift_e up e) as [? ?] eqn:?; simpl in *
   end.
 
+(*
 Ltac translateControlDecl_destr := 
   match goal with
   | |- context [TranslateControlDecl ?cd ?env]
@@ -61,254 +67,177 @@ Ltac translateTopDecl_destr :=
   | |- context [TranslateTopDecl ?td ?env]
     => destruct (TranslateTopDecl td env) as [? ?] eqn:?; simpl in *
   end.
-
-Ltac transformExpr_destr_hyp :=
+*)
+Ltac lift_e_destr_hyp :=
   match goal with
-  | H: context [TransformExpr ?e ?env] |- _
-    => destruct (TransformExpr e env)
-      as [[? ?] ?] eqn:?; simpl in *
+  | H: context [lift_e ?up ?e] |- _
+    => destruct (lift_e up e)
+      as [? ?] eqn:?; simpl in *
   end.
 
-Ltac transformExpr_destr_hyp_rewrite :=
+Ltac lift_e_destr_hyp_rewrite :=
   match goal with
-  | H: TransformExpr ?e ?env = (_,_,_),
-       Hy : context [TransformExpr ?e ?env]
+  | H: lift_e ?up ?e = (_,_),
+      Hy : context [lift_e ?up ?e]
     |- _ => rewrite H in Hy; simpl in *
   end.
 
+Inductive lifted_expr : Expr.e -> Prop :=
+| lifted_bool (b : bool) :
+  lifted_expr b
+| lifted_var τ x :
+  lifted_expr (Expr.Var τ x)
+| lifted_member τ e x :
+  lifted_expr e ->
+  lifted_expr (Expr.Member τ x e)
+| lifted_error err :
+  lifted_expr (Expr.Error err).
 
-(*Ltac quantify_varNameGen :=
-  match goal with
-        | env: VarNameGen.t, H: (forall _: VarNameGen.t, _)
-      |-   _ => specialize H with env
-    end.*) 
+Definition lifted_args (args : Expr.args) : Prop :=
+  Forall (pred_paramarg_same lifted_expr) args.
 
-Ltac fold_destr :=
-  match goal with
-  | |- context [fold_left ?f ?l ?acc]
-    => destruct (fold_left f l acc) as [[? ?] ?] eqn:Hfoldl; simpl in *
-  | |- context [fold_right ?f ?acc ?l]
-    => destruct (fold_right f acc l) as [[? ?] ?] eqn:Hfoldl; simpl in *
-  end.
+Variant lifted_lexpr : Expr.e -> Prop :=
+  | lifted_lifted_expr e :
+    lifted_expr e ->
+    lifted_lexpr e
+  | lifted_bit w n :
+    lifted_lexpr (Expr.Bit w n)
+  | lifted_int w z :
+    lifted_lexpr (Expr.Int w z)
+  | lifted_slice e hi lo :
+    lifted_expr e ->
+    lifted_lexpr (Expr.Slice e hi lo)
+  | lifted_cast τ e :
+    lifted_expr e ->
+    lifted_lexpr (Expr.Cast τ e)
+  | lifted_uop τ op e :
+    lifted_expr e ->
+    lifted_lexpr (Expr.Uop τ op e)
+  | lifted_bop τ op e₁ e₂ :
+    lifted_expr e₁ ->
+    lifted_expr e₂ ->
+    lifted_lexpr (Expr.Bop τ op e₁ e₂)
+  | lift_struct es ob :
+    Forall lifted_expr es ->
+    lifted_lexpr (Expr.Struct es ob).
 
-Section Lifted.
-  Arguments String.append : simpl never.
+Variant lifted_fun_kind : Stmt.fun_kind -> Prop :=
+  | lifted_Funct x τs oe :
+    predop lifted_expr oe ->
+    lifted_fun_kind (Stmt.Funct x τs oe)
+  | lifted_Action x es :
+    Forall lifted_expr es ->
+    lifted_fun_kind (Stmt.Action x es)
+  | lifted_Method x m τs oe :
+    predop lifted_expr oe ->
+    lifted_fun_kind (Stmt.Method x m τs oe).
+
+Variant lifted_parser_expr : Parser.e -> Prop :=
+  | lifted_goto st : 
+    lifted_parser_expr (Parser.Goto st)
+  | lifted_select exp default cases : 
+    lifted_expr exp ->
+    lifted_parser_expr (Parser.Select exp default cases).
+
+Inductive lifted_stmt : Stmt.s -> Prop :=
+| lifted_skip :
+  lifted_stmt Stmt.Skip
+| lifted_vardecl te s :
+  match te with
+  | inl t => True
+  | inr e => lifted_lexpr e
+  end ->
+  lifted_stmt s ->
+  lifted_stmt (Stmt.Var te s)
+| lifted_assign e1 e2 :
+  lifted_expr e1 ->
+  lifted_expr e2 ->
+  lifted_stmt (Stmt.Assign e1 e2)
+| lifted_cond e s1 s2 :
+  lifted_expr e ->
+  lifted_stmt s1 ->
+  lifted_stmt s2 ->
+  lifted_stmt (Stmt.Conditional e s1 s2)
+| lifted_seq s1 s2 :
+  lifted_stmt s1 ->
+  lifted_stmt s2 ->
+  lifted_stmt (Stmt.Seq s1 s2)
+| lifted_call fk args :
+  lifted_fun_kind fk ->
+  lifted_args args ->
+  lifted_stmt (Stmt.Call fk args)
+| lifted_return eo :
+  match eo with
+  | Some e => lifted_expr e
+  | None   => True
+  end ->
+  lifted_stmt (Stmt.Return eo)
+| lifted_exit :
+  lifted_stmt Stmt.Exit
+| lifted_transition e :
+  lifted_parser_expr e ->
+  lifted_stmt (Stmt.Transition e)
+| lifted_invoke t :
+  lifted_stmt (Stmt.Invoke t)
+| lifted_apply x ext_args args :
+  lifted_args args ->
+  lifted_stmt (Stmt.Apply x ext_args args).
+
+Variant lifted_control_Decl : Control.d -> Prop :=
+  | lifted_Decl_Action act cps dps body :
+    lifted_stmt body ->
+    lifted_control_Decl (Control.Action act cps dps body)
+  | lifted_Table table_name key actions :
+    Forall lifted_expr (map fst key) ->
+    lifted_control_Decl (Control.Table table_name key actions).
+
+Inductive lifted_top_Decl : TopDecl.d -> Prop :=
+| lifted_Instantiate c_name type_args cargs :
+  lifted_top_Decl (TopDecl.Instantiate c_name type_args cargs)
+| lifted_Extern e_name type_params c_params methods : 
+  lifted_top_Decl (TopDecl.Extern e_name type_params c_params methods)
+| lifted_Control c cparams eps params body apply_blk :
+  Forall lifted_control_Decl body -> lifted_stmt apply_blk ->
+  lifted_top_Decl (TopDecl.Control c cparams eps params body apply_blk)
+| lifted_Parser p cparams eps params start_state states :
+  lifted_stmt start_state -> Forall lifted_stmt states ->
+  lifted_top_Decl (TopDecl.Parser p cparams eps params start_state states)
+| lifted_Function f tparams signature body :
+  lifted_stmt body -> lifted_top_Decl (TopDecl.Funct f tparams signature body).
+
+Local Hint Constructors lifted_expr : core.
+Local Hint Constructors lifted_lexpr : core.
+Local Hint Constructors lifted_parser_expr : core.
   
-  Context {tags_t : Type}.
-  
-  Inductive lifted_expr : Expr.e tags_t -> Prop :=
-  | lifted_bool b i :
-      lifted_expr <{ BOOL b @ i }>
-  | lifted_var x τ i :
-      lifted_expr <{ Var x:τ @ i }>
-  | lifted_member τ e x i :
-      lifted_expr e ->
-      lifted_expr <{ Mem e dot x : τ @ i }>
-  | lifted_error err i :
-      lifted_expr <{ Error err @ i }>
-  | lifted_access ts e z i :
-      lifted_expr e ->
-      lifted_expr <{ Access e[z] : ts @ i }>.
+Lemma lift_e_lifted_expr : forall e E l up,
+    lift_e up e = (l, E) ->
+    Forall lifted_lexpr l /\ lifted_expr E.
+Proof.
+  intro e; induction e using custom_e_ind;
+    intros E l up h; unravel in *;
+    repeat lift_e_destr;
+    try lift_e_destr_hyp;
+    repeat pair_destr; auto.
+  - apply IHe in Heqp as [? ?]; auto.
+  - apply IHe in Heqp as [? ?]; auto.
+  - apply IHe in Heqp as [? ?]; auto.
+  - destruct (lift_e (List.length l0 + up) e2) as [l2  e2'] eqn:eql2.
+    apply IHe1 in Heqp as [? ?].
+    apply IHe2 in eql2 as [? ?].
+    pair_destr.
+    split; auto.
+    constructor.
+    + apply lifted_bop; auto.
+      admit (* TODO: prove shifting preserves lifting. *).
+    + rewrite Forall_app; auto.
+  - (* TODO *)
+Admitted.
 
-  Definition lifted_args (args : Expr.arrowE tags_t) : Prop :=
-    F.predfs_data (pred_paramarg_same lifted_expr) (paramargs args) /\
-    predop lifted_expr (rtrns args).
-  
-  Inductive lifted_stmt : Stmt.s tags_t -> Prop :=
-  | lifted_skip i :
-      lifted_stmt -{ skip @ i }-
-  | lifted_vardecl x te i :
-      match te with
-      | inl t => True
-      | inr e => lifted_expr e
-      end ->
-      lifted_stmt -{ var x with te @ i }-
-  | lifted_assign e1 e2 i :
-      lifted_expr e1 ->
-      lifted_expr e2 ->
-      lifted_stmt -{ asgn e1 := e2 @ i }-
-  | lifted_bit x w n i iw :
-      lifted_stmt -{ init x := w W n @ iw @ i }-
-  | lifted_int x w z i iw :
-      lifted_stmt -{ init x := w S z @ iw @ i }-
-  | lifted_uop τ op x e i ie :
-      lifted_expr e ->
-      lifted_stmt -{ init x := UOP op e : τ @ ie @ i}-
-  | lifted_bop τ op x e1 e2 i ie1e2 :
-      lifted_expr e1 ->
-      lifted_expr e2 ->
-      lifted_stmt -{ init x := BOP e1 op e2 : τ @ ie1e2 @ i }-
-  | lifted_slice x e hi lo i ie :
-      lifted_expr e ->
-      lifted_stmt -{ init x := Slice e [hi:lo] @ ie @ i }-
-  | lifted_cast x e τe i ie :
-      lifted_expr e ->
-      lifted_stmt -{ init x := Cast e:τe @ ie @ i }-
-  | lifted_tuple x es i ies :
-      Forall lifted_expr es ->
-      lifted_stmt -{ init x := tup es @ ies @ i }-
-  | lifted_struct x es i ies :
-      F.predfs_data lifted_expr es ->
-      lifted_stmt -{ init x := struct { es } @ ies @ i }-
-  | lifted_header x e es i ies :
-      lifted_expr e ->
-      F.predfs_data lifted_expr es ->
-      lifted_stmt -{ init x := hdr { es } valid:=e @ ies @ i }-
-  | lifted_stack x es ni τs i ies :
-      Forall lifted_expr es ->
-      lifted_stmt -{ init x := Stack es:τs nextIndex:=ni @ ies @ i }-
-  | lifted_cond e s1 s2 i :
-      lifted_expr e ->
-      lifted_stmt s1 ->
-      lifted_stmt s2 ->
-      lifted_stmt -{ if e then s1 else s2 @ i }-
-  | lifted_seq s1 s2 i :
-      lifted_stmt s1 ->
-      lifted_stmt s2 ->
-      lifted_stmt -{ s1; s2 @ i }-
-  | lifted_block s :
-      lifted_stmt s ->
-      lifted_stmt -{ b{ s }b }-
-  | lifted_extern_method_call e f targs args i :
-      lifted_args args ->
-      lifted_stmt (Stmt.SExternMethodCall e f targs args i)
-  | lifted_fun_call f targs args i :
-      lifted_args args ->
-      lifted_stmt (Stmt.SFunCall f targs args i)
-  | lifted_act_call a args i :
-      F.predfs_data (pred_paramarg_same lifted_expr) args ->
-      lifted_stmt -{ calling a with args @ i }-
-  | lifted_return eo i :
-      match eo with
-      | Some e => lifted_expr e
-      | None   => True
-      end ->
-      lifted_stmt -{ return eo @ i }-
-  | lifted_exit i :
-      lifted_stmt -{ exit @ i }-
-  | lifted_invoke t i :
-      lifted_stmt -{ invoke t @ i }-
-  | lifted_apply x ext_args args i :
-      F.predfs_data (pred_paramarg_same lifted_expr) args ->
-      lifted_stmt -{ apply x with ext_args & args @ i }-
-  | lifted_headerStackOp hdr_stk_name typ op n i :
-      lifted_stmt (Stmt.SHeaderStackOp hdr_stk_name typ op n i)
-  | lifted_setValidity e validity i : 
-      lifted_expr e -> lifted_stmt (Stmt.SSetValidity e validity i).
-  
-  Local Hint Constructors lifted_expr : core.
-
-  Inductive lifted_parser_expr : Parser.e tags_t -> Prop :=
-  | lifted_goto st i : 
-      lifted_parser_expr (Parser.PGoto st i)
-  | lifted_select exp default cases i: 
-      lifted_expr exp -> lifted_parser_expr default -> 
-      Field.predfs_data lifted_parser_expr cases ->
-      lifted_parser_expr (Parser.PSelect exp default cases i).
-
-  Local Hint Constructors lifted_parser_expr : core.
-  
-  Definition lifted_parser_state (stblk : Parser.state_block tags_t) : Prop :=
-    lifted_stmt (Parser.stmt stblk) /\ lifted_parser_expr (Parser.trans stblk).
-  
-  Definition lifted_parser_states (states: F.fs string (Parser.state_block tags_t)) : Prop := 
-    F.predfs_data lifted_parser_state states.
-
-  (*Check lifted_parser_states.*)
-  Definition lifted_table (tbl : Control.table tags_t) : Prop :=
-    Forall (fun '(e, _) => lifted_expr e) (Control.table_key tbl).
-  
-  Inductive lifted_control_Decl : Control.d tags_t -> Prop :=
-  | lifted_CDAction act sig body i :
-      lifted_stmt body ->
-      lifted_control_Decl (Control.CDAction act sig body i)
-  | lifted_CDTable table_name body i :
-      lifted_table body ->
-      lifted_control_Decl (Control.CDTable table_name body i)
-  | lifted_CDSeq d1 d2 i :
-      lifted_control_Decl d1 -> lifted_control_Decl d2 ->
-      lifted_control_Decl (Control.CDSeq d1 d2 i).
-
-  Inductive lifted_top_Decl : TopDecl.d tags_t -> Prop :=
-  | lifted_TPInstantiate c_name i_name type_args cargs i :
-      lifted_top_Decl (TopDecl.TPInstantiate c_name i_name type_args cargs i)
-  | lifted_TPExtern e_name type_params c_params methods i : 
-      lifted_top_Decl (TopDecl.TPExtern e_name type_params c_params methods i)
-  | lifted_TPControl c cparams eps params body apply_blk i :
-      lifted_control_Decl body -> lifted_stmt apply_blk ->
-      lifted_top_Decl (TopDecl.TPControl c cparams eps params body apply_blk i)
-  | lifted_TPParser p cparams eps params start_state states i :
-      lifted_parser_state start_state -> lifted_parser_states states ->
-      lifted_top_Decl (TopDecl.TPParser p cparams eps params start_state states i)
-  | lifted_TPFunction f tparams signature body i :
-      lifted_stmt body -> lifted_top_Decl (TopDecl.TPFunction f tparams signature body i)
-  | lifted_TPSeq d1 d2 i :
-      lifted_top_Decl d1 -> lifted_top_Decl d2 ->
-      lifted_top_Decl (TopDecl.TPSeq d1 d2 i).
-
-  Section HelperLemmas.
-    Variable f :
-      Expr.e tags_t -> VarNameGen.t ->
-      Stmt.s tags_t * Expr.e tags_t * VarNameGen.t.
-      
-    Section General.
-      Hypothesis Hf : forall e env, lifted_expr (snd (fst (f e env))).
-      
-      Lemma TransformExprList'_lifted_expr :
-        forall es env i,
-          Forall
-            lifted_expr
-            (snd (fst (TransformExprList' f es env i))).
-      Proof.
-        unfold TransformExprList'.
-        intro es; induction es as [| e es IHes];
-          intros env i; simpl; auto.
-        fold_destr. destruct (f e t) as [[s' e'] env'] eqn:Heqfet.
-        constructor.
-        - apply f_equal with (f:=snd ∘ fst) in Heqfet; unravel in *.
-          rewrite <- Heqfet; auto.
-        - specialize IHes with env i.
-          rewrite Hfoldl in IHes; auto.
-      Qed.
-      
-      Lemma TransformFields'_lifted_expr :
-        forall es env i,
-          F.predfs_data
-            lifted_expr
-            (snd (fst (TransformFields' f es env i))).
-      Proof.
-        unfold TransformFields', Field.fold.
-        intro es; induction es as [| (x & e) es IHes];
-          intros env i; unfold F.predfs_data, F.predf_data in *;
-            unravel in *; auto; fold_destr.
-        destruct (f e t) as [[s' e'] env'] eqn:Heqfet; unravel.
-        constructor; unravel.
-        - apply f_equal with (f:=snd ∘ fst) in Heqfet;
-            unravel in *. rewrite <- Heqfet; auto.
-        - specialize IHes with env i.
-          rewrite Hfoldl in IHes; auto.
-      Qed.
-    End General.
-  End HelperLemmas.
-
-  Local Hint Resolve TransformExprList'_lifted_expr : core.
-  Local Hint Resolve TransformFields'_lifted_expr : core.
-  
-  Lemma TransformExpr_lifted_expr : forall e env,
-      lifted_expr (snd (fst (TransformExpr e env))).
-  Proof.
-    intro e; induction e using custom_e_ind;
-      intro env; unravel in *;
-        repeat transformExpr_destr; auto;
-          try (constructor; specialize IHe with env;
-               transformExpr_destr_hyp; inv Heqp; auto; assumption).
-  Qed.
-  
-  Local Hint Constructors lifted_stmt : core.
+Local Hint Constructors lifted_stmt : core.
 
   Ltac seq_lift :=
     match goal with
-    | |- lifted_stmt -{ _; _ @ _ }-
+    | |- lifted_stmt (_; _ @ _ }-
       => apply lifted_seq
     end.
 
@@ -341,7 +270,7 @@ Section Lifted.
     forall es,
       Forall
         (fun e => forall env,
-             lifted_stmt (fst (fst (TransformExpr e env)))) es ->
+             lifted_stmt (fst (fst (lift_e up e)))) es ->
       forall env i,
         lifted_stmt (fst (fst (TransformExprList' TransformExpr es env i))).
   Proof.
@@ -361,7 +290,7 @@ Section Lifted.
     forall fields,
       F.predfs_data
         (fun e => forall env,
-             lifted_stmt (fst (fst (TransformExpr e env)))) fields ->
+             lifted_stmt (fst (fst (lift_e up e)))) fields ->
       forall env i,
         lifted_stmt (fst (fst (TransformFields' TransformExpr fields env i))).
   Proof.
@@ -378,7 +307,7 @@ Section Lifted.
   Local Hint Resolve TransformFields'_lifted_stmt_Forall : core.
   
   Lemma TransformExpr_lifted_stmt : forall e env,
-      lifted_stmt (fst (fst (TransformExpr e env))).
+      lifted_stmt (fst (fst (lift_e up e))).
   Proof.
     intro e; induction e using custom_e_ind;
       intro env; unravel in *;
@@ -441,7 +370,7 @@ Section Lifted.
     apply f_equal with (f := fst) in Heqp; apply f_equal with (f := snd) in Heqp; simpl in Heqp;
       rewrite <- Heqp; auto.
 
-  Lemma TranslateArgs_lifted_stmt : forall (a : Expr.args tags_t) env i,
+  Lemma TranslateArgs_lifted_stmt : forall (a : Expr.args ) env i,
   lifted_stmt (fst (fst (TranslateArgs a env i))).
   Proof.
     intros a i. induction a;
@@ -455,7 +384,7 @@ Section Lifted.
 
   Local Hint Resolve TranslateArgs_lifted_stmt : core.
 
-  Lemma TranslateArrowE_lifted_stmt : forall (args : Expr.arrowE tags_t) env i, 
+  Lemma TranslateArrowE_lifted_stmt : forall (args : Expr.arrowE ) env i, 
   lifted_stmt (fst (fst (TranslateArrowE args env i))).
   Proof.
     intros [pas returns] i env; simpl.
@@ -483,7 +412,7 @@ Section Lifted.
 
   Local Hint Constructors predop : core.
 
-  Lemma TransformExpr_lifted_args : forall pas i (e:Expr.e tags_t) t env,
+  Lemma TransformExpr_lifted_args : forall pas i (e:Expr.e ) t env,
       lifted_args {|paramargs:=snd (fst (TranslateArgs pas i env));
                     rtrns:=Some (snd (fst (TransformExpr e t)))|}.
   Proof.
@@ -493,7 +422,7 @@ Section Lifted.
 
   Local Hint Resolve TransformExpr_lifted_args : core.
    
-  Lemma TranslateArrowE_lifted_args : forall (args : Expr.arrowE tags_t) env i, 
+  Lemma TranslateArrowE_lifted_args : forall (args : Expr.arrowE ) env i, 
   lifted_args (snd (fst (TranslateArrowE args env i))).
   Proof.
     intros [pas returns] i env; simpl.
@@ -505,7 +434,7 @@ Section Lifted.
 
   Local Hint Resolve TranslateArrowE_lifted_args : core.
 
-  Lemma TranslateStmt_lifted_stmt : forall (s : Stmt.s tags_t) (env:VarNameGen.t),
+  Lemma TranslateStmt_lifted_stmt : forall (s : Stmt.s ) (env:VarNameGen.t),
   lifted_stmt (fst (TranslateStatement s env)).
   Proof.
   intros s. induction s; intros env; try simpl; auto; repeat transformExpr_destr.
@@ -523,12 +452,12 @@ Section Lifted.
     + hyp_f_equal_fst Heqp.
     + constructor. 
       * hyp_f_equal_snd Heqp. 
-      * hyp_f_equal Heqp0 (fun x:(Stmt.s tags_t) => x).
-      * hyp_f_equal Heqp1 (fun x:(Stmt.s tags_t) => x). 
+      * hyp_f_equal Heqp0 (fun x:(Stmt.s ) => x).
+      * hyp_f_equal Heqp1 (fun x:(Stmt.s ) => x). 
   - repeat translateStmt_destr. constructor. 
-    + hyp_f_equal Heqp (fun x:(Stmt.s tags_t) => x).
-    + hyp_f_equal Heqp0 (fun x:(Stmt.s tags_t) => x). 
-  - translateStmt_destr. constructor. hyp_f_equal Heqp (fun x:(Stmt.s tags_t) => x).
+    + hyp_f_equal Heqp (fun x:(Stmt.s ) => x).
+    + hyp_f_equal Heqp0 (fun x:(Stmt.s ) => x). 
+  - translateStmt_destr. constructor. hyp_f_equal Heqp (fun x:(Stmt.s ) => x).
   - translateArrowE_destr. constructor.
     + hyp_f_equal_fst Heqp.
     + constructor. hyp_f_equal_snd Heqp. 
@@ -554,10 +483,10 @@ Section Lifted.
   Local Hint Resolve TranslateStmt_lifted_stmt : core.
 
 
-  Lemma TranslateCases_lifted_stmt : forall (translateParserE : Parser.e tags_t -> VarNameGen.t -> (Stmt.s tags_t) * Parser.e tags_t * VarNameGen.t)
-  (cases: Field.fs Parser.pat (Parser.e tags_t)),
+  Lemma TranslateCases_lifted_stmt : forall (translateParserE : Parser.e  -> VarNameGen.t -> (Stmt.s ) * Parser.e  * VarNameGen.t)
+  (cases: Field.fs Parser.pat (Parser.e )),
   F.predfs_data (fun pe => forall env, lifted_stmt (fst (fst (translateParserE pe env)))) cases -> 
-  forall (env: VarNameGen.t) (i : tags_t), 
+  forall (env: VarNameGen.t) (: ), 
   lifted_stmt (fst (fst (TranslateCases' translateParserE cases env i))).
   Proof.
   intros translateParserE cases Hpte; ind_list_predfs; intros. 
@@ -570,7 +499,7 @@ Section Lifted.
 
   Local Hint Resolve TranslateCases_lifted_stmt : core.
 
-  Lemma TranslateParserExpr_lifted_stmt : forall (e : Parser.e tags_t) (env:VarNameGen.t),
+  Lemma TranslateParserExpr_lifted_stmt : forall (e : Parser.e ) (env:VarNameGen.t),
   lifted_stmt (fst (fst (TranslateParserExpr e env))).
   Proof.
   intros e. induction e using pe_ind; intro env; try simpl; auto.
@@ -583,10 +512,10 @@ Section Lifted.
 
   Local Hint Resolve TranslateParserExpr_lifted_stmt : core.
 
-  Lemma TranslateCases_lifted_expr : forall (translateParserE : Parser.e tags_t -> VarNameGen.t -> (Stmt.s tags_t) * Parser.e tags_t * VarNameGen.t)
-  (cases: Field.fs Parser.pat (Parser.e tags_t)),
+  Lemma TranslateCases_lifted_expr : forall (translateParserE : Parser.e  -> VarNameGen.t -> (Stmt.s ) * Parser.e  * VarNameGen.t)
+  (cases: Field.fs Parser.pat (Parser.e )),
   F.predfs_data (fun pe => forall env, lifted_parser_expr (snd (fst (translateParserE pe env)))) cases -> 
-  forall (env: VarNameGen.t) (i : tags_t), 
+  forall (env: VarNameGen.t) (: ), 
   F.predfs_data lifted_parser_expr (snd (fst (TranslateCases' translateParserE cases env i))).
   Proof.
   intros translateParserE cases Hpte; ind_list_predfs; intros; unfold F.predfs_data in *; 
@@ -599,7 +528,7 @@ Section Lifted.
 
   Local Hint Resolve TranslateCases_lifted_expr : core.
 
-  Lemma TranslateParserExpr_lifted_parser_expr : forall (e : Parser.e tags_t) (env:VarNameGen.t),
+  Lemma TranslateParserExpr_lifted_parser_expr : forall (e : Parser.e ) (env:VarNameGen.t),
   lifted_parser_expr (snd (fst (TranslateParserExpr e env))).
   Proof.
   intros e. induction e using pe_ind; intro env; try simpl; auto.
@@ -613,12 +542,12 @@ Section Lifted.
   Local Hint Resolve TranslateParserExpr_lifted_parser_expr : core.
 
   Lemma TranslateParserState_lifted_stmt :
-    forall (parser_state: Parser.state_block tags_t) (env : VarNameGen.t),
+    forall (parser_state: Parser.state_block ) (env : VarNameGen.t),
       lifted_parser_state (fst (TranslateParserState parser_state env)).
   Proof.
     intros [s e] env; simpl; translateStmt_destr; translateParserExpr_destr.
     destruct p. simpl. unfold lifted_parser_state; split; cbn; try constructor.
-    - hyp_f_equal Heqp (fun x:(Stmt.s tags_t) => x).
+    - hyp_f_equal Heqp (fun x:(Stmt.s ) => x).
     - hyp_f_equal_fst Heqp0.
     - hyp_f_equal_snd Heqp0.
   Qed.
@@ -626,7 +555,7 @@ Section Lifted.
   Local Hint Resolve TranslateParserState_lifted_stmt : core.
 
   Lemma TranslateParserStates_lifted_stmt :
-    forall (parser_states: Field.fs string (Parser.state_block tags_t)) (env : VarNameGen.t),
+    forall (parser_states: Field.fs string (Parser.state_block )) (env : VarNameGen.t),
       lifted_parser_states (fst (TranslateParserStates parser_states env)).
   Proof.
     induction parser_states; intros; simpl in *.
@@ -652,7 +581,7 @@ Section Lifted.
   Local Hint Resolve TranslateParserStates_lifted_stmt : core.
 
   Lemma TranslateTable_lifted_stmt :
-    forall (t: Control.table tags_t) (env: VarNameGen.t) (i : tags_t),
+    forall (t: Control.table ) (env: VarNameGen.t) (: ),
       lifted_stmt (fst (fst (TranslateTable t env i))).
   Proof.
     intros [ky acts] env i; cbn; fold_destr; clear acts.
@@ -669,7 +598,7 @@ Section Lifted.
   Local Hint Resolve TranslateTable_lifted_stmt : core.
 
   Lemma TranslateTable_lifted_table :
-    forall (t: Control.table tags_t) (env: VarNameGen.t) (i : tags_t),
+    forall (t: Control.table ) (env: VarNameGen.t) (: ),
       lifted_table (snd (fst (TranslateTable t env i))).
   Proof.
     intros [ky acts] env i; cbn; fold_destr.
@@ -688,7 +617,7 @@ Section Lifted.
 
   Local Hint Resolve TranslateTable_lifted_table : core.
 
-  Lemma TranslateControlDecl_lifted_stmt : forall (cd : Control.d tags_t) (env : VarNameGen.t),
+  Lemma TranslateControlDecl_lifted_stmt : forall (cd : Control.d ) (env : VarNameGen.t),
       lifted_stmt (fst (fst (TranslateControlDecl cd env))).
   Proof.
     intro cd. induction cd; intro env; simpl; auto.  
@@ -701,7 +630,7 @@ Section Lifted.
 
   Local Hint Resolve TranslateControlDecl_lifted_stmt : core.
 
-  Lemma TranslateControlDecl_lifted_decl : forall (cd : Control.d tags_t) (env : VarNameGen.t),
+  Lemma TranslateControlDecl_lifted_decl : forall (cd : Control.d ) (env : VarNameGen.t),
       lifted_control_Decl (snd (fst (TranslateControlDecl cd env))).
   Proof.
     intro cd. induction cd; intro env; simpl; auto.  
@@ -720,7 +649,7 @@ Section Lifted.
   
   Local Hint Resolve TranslateControlDecl_lifted_decl : core.
 
-  Lemma TranslateTopDecl_lifted_top_Decl : forall (td : TopDecl.d tags_t) (env : VarNameGen.t),
+  Lemma TranslateTopDecl_lifted_top_Decl : forall (td : TopDecl.d ) (env : VarNameGen.t),
       lifted_top_Decl (fst (TranslateTopDecl td env)).
   Proof.
     induction td; intros; simpl; try solve [constructor].
@@ -762,7 +691,7 @@ Section Lifted.
 
   Local Hint Resolve TranslateTopDecl_lifted_top_Decl : core.
 
-  Lemma TranslateProgram_lifted_top_Decl : forall (prog: TopDecl.d tags_t),
+  Lemma TranslateProgram_lifted_top_Decl : forall (prog: TopDecl.d ),
       lifted_top_Decl (TranslateProgram prog).
   Proof.
     unfold TranslateProgram.
